

THE UNIVERSITY OF HONG KONG  
DEPARTMENT OF MATHEMATICS

MATH6101 / MATH7101: Intermediate Complex Analysis  
**Holomorphic Immersion via Poincaré Series**

**Proposition.** *Let  $X = \Delta/\Gamma$  be a compact Riemann surface of genus  $g \geq 2$ . Let  $x_0 \in \Delta$ . Then there exists an integer  $k \geq 2$ , and bounded holomorphic functions  $t, s \in H^\infty(\Delta)$  such that*

(a)  $f := P_\Gamma^k(t)$  satisfies  $f(x_0) \neq 0$

(b)  $g := P_\Gamma^k(s)$  satisfies  $\left(\frac{g}{f}\right)'(x_0) \neq 0$

*Proof.* Define  $\Gamma_0 \subset \Gamma$  by  $\Gamma_0 := \left\{ \gamma \in \Gamma : |\gamma'(x_0)| \geq \frac{1}{2} \right\}$ . By the proof of the convergence of Poincaré series for  $k = 2$ , we have  $S := \sum_{\gamma \in \Gamma} |\gamma'(x_0)|^2 < \infty$ . Hence, the subset  $\Gamma_0 \subset \Gamma$  is finite. Enumerate  $\Gamma_0$  as  $\Gamma_0 = \{\gamma_1, \gamma_2, \dots, \gamma_N\}$  where  $\gamma_1 = \text{id}$ . Consider the following two polynomials.

$$P(z) = \prod_{i=2}^N (z - \gamma_i x_0)^2$$

$$Q(z) = (z - x_0) \prod_{i=2}^N (z - \gamma_i x_0)^2.$$

Since  $\gamma x_0 \neq x_0$  for any  $\gamma \in \Gamma - \{\text{id}\}$ , we have  $P(x_0) \neq 0$ . Clearly  $Q(x_0) = 0$ . Moreover,  $Q(z) = (z - x_0)P(z)$  hence

$$Q'(z) = P(z) + (z - x_0)P'(z),$$

so that  $Q'(x_0) = P(x_0) \neq 0$ . Thus,  $(P(x_0), P'(x_0))$ , and  $(Q(x_0), Q'(x_0))$ , are linearly independent, from which we deduce readily

(#) Given any complex numbers  $a, b \in \mathbb{C}$ , there exists a polynomial  $R(z) = \alpha P(z) + \beta Q(z)$  for some  $\alpha, \beta \in \mathbb{C}$ , such that  $R(x_0) = a, R'(x_0) = b$ .

We consider special cases of (#). Let  $A(z)$  be the polynomial given in (#) such that  $A(x_0) = 1, A'(x_0) = 0$ , and let  $B(z)$  be the polynomial given in (#) satisfying  $B(x_0) = 0, B'(x_0) = 1$ . Denote now by  $t := A|_\Delta \in H^\infty(\Delta), s := B|_\Delta \in H^\infty(\Delta)$ . We claim that for  $k$  sufficiently large,  $f := P_\Gamma^k(t), g := P_\Gamma^k(s)$  satisfy the requirements in the proposition.

Noting that  $t(\gamma_i x_0) = 0$  for  $2 \leq i \leq N$ , we have

$$\begin{aligned} f(x_0) &= \sum_{\gamma \in \Gamma_0} t(\gamma x_0) (\gamma'(x_0))^k + \sum_{\gamma \in \Gamma - \Gamma_0} t(\gamma x_0) (\gamma'(x_0))^k, \\ &= 1 + \sum_{\gamma \in \Gamma - \Gamma_0} t(\gamma x_0) (\gamma'(x_0))^k, \end{aligned}$$

so that

$$|f(x_0) - 1| \leq \sum_{\gamma \in \Gamma - \Gamma_0} |t(\gamma x_0)| |\gamma'(x_0)|^k.$$

Since  $t$  is bounded on  $\Delta$ , there exists  $M > 0$  such that  $|t(\gamma x_0)| \leq M$  for any  $\gamma \in \Gamma$ . Recall that  $S := \sum_{\gamma \in \Gamma} |\gamma'(x_0)|^2 < \infty$ . Hence,

$$\begin{aligned} |f(x_0) - 1| &\leq M \sum_{\gamma \in \Gamma - \Gamma_0} |\gamma'(x_0)|^k = M \sum_{\gamma \in \Gamma - \Gamma_0} |\gamma'(x_0)|^2 |\gamma'(x_0)|^{k-2} \\ &\leq M \left( \sum_{\gamma \in \Gamma} |\gamma'(x_0)|^2 \right) \left( \sup_{\gamma \in \Gamma - \Gamma_0} |\gamma'(x_0)| \right)^{k-2} \leq MS \left( \frac{1}{2} \right)^{k-2}. \end{aligned}$$

Choose  $k_0$  such that  $MS \left( \frac{1}{2} \right)^{k_0-2} < \frac{1}{2}$ . Then, for any  $k \geq k_0$ , we have  $|f(x_0) - 1| < \frac{1}{2}$ , hence  $|f(x_0)| > \frac{1}{2}$ . In particular,  $f(x_0) \neq 0$ .

For the function  $g$  we want to estimate  $\left( \frac{g}{f} \right)'(x_0)$ . Now

$$\left( \frac{g}{f} \right)'(x_0) = \frac{1}{(f(x_0))^2} (f(x_0)g'(x_0) - g(x_0)f'(x_0)).$$

Hence,

$$\begin{aligned} f'(x_0) &= \sum_{\gamma \in \Gamma_0} t'(\gamma x_0) (\gamma'(x_0))^k + \sum_{\gamma \in \Gamma_0} kt(\gamma x_0) (\gamma'(x_0))^{k-1} \gamma''(x_0) \\ &\quad + \sum_{\gamma \in \Gamma - \Gamma_0} t'(\gamma x_0) (\gamma'(x_0))^k + \sum_{\gamma \in \Gamma - \Gamma_0} kt(\gamma x_0) (\gamma'(x_0))^{k-1} \gamma''(x_0). \end{aligned}$$

Note that by Cauchy estimates there exists a constant  $C$  such that  $|\gamma''(x_0)| \leq C$  for any  $\gamma \in \Gamma$ . By our choice of  $t = A|_\Delta$  we have  $t(\gamma_i x_0) = t'(\gamma_i x_0) = 0$  for  $2 \leq i \leq N$ , while  $t(x_0) = 1, t'(x_0) = 0$ . Moreover for  $\gamma = \text{id}$ ,  $\gamma'' = 0$ . Hence,

$$f'(x_0) = \sum_{\gamma \in \Gamma - \Gamma_0} t'(\gamma x_0) (\gamma'(x_0))^k + k \sum_{\gamma \in \Gamma - \Gamma_0} t(\gamma x_0) (\gamma'(x_0))^{k-1} \gamma''(x_0).$$

Writing  $(\gamma'(x_0))^k = (\gamma'(x_0))^2 (\gamma'(x_0))^{k-2}$  and  $(\gamma'(x_0))^{k-1} = (\gamma'(x_0))^2 (\gamma'(x_0))^{k-3}$  we have

$$|f'(x_0)| \leq \sup_{\Delta} |t'(z)| \cdot S\left(\frac{1}{2}\right)^{k-2} + k \sup_{\Delta} |t(z)| \cdot S\left(\frac{1}{2}\right)^{k-3} \cdot C. \quad (1)$$

Our task is to prove that  $\left(\frac{g}{f}\right)'(x_0) \neq 0$  for  $k$  sufficiently large. Given that  $s(x_0) = 0, s'(x_0) = 1, s(\gamma_i x_0) = s'(\gamma_i x_0) = 0$  for  $2 \leq i \leq N$ , we have

$$\begin{aligned} g(x_0) &= \sum_{\gamma \in \Gamma_0} s(\gamma x_0) (\gamma'(x_0))^k + \sum_{\gamma \in \Gamma - \Gamma_0} s(\gamma x_0) (\gamma'(x_0))^k \\ &= \sum_{\gamma \in \Gamma - \Gamma_0} s(\gamma x_0) (\gamma'(x_0))^k, \end{aligned}$$

so that

$$|g(x_0)| \leq \sup_{\Delta} |s(z)| \cdot S\left(\frac{1}{2}\right)^{k-2}. \quad (2)$$

Moreover,

$$\begin{aligned} g'(x_0) &= \sum_{\gamma \in \Gamma_0} s'(\gamma x_0) (\gamma'(x_0))^k + \sum_{\gamma \in \Gamma_0} k s(\gamma x_0) (\gamma'(x_0))^{k-1} \gamma''(x_0) \\ &\quad + \sum_{\gamma \in \Gamma - \Gamma_0} s'(\gamma x_0) (\gamma'(x_0))^k + \sum_{\gamma \in \Gamma - \Gamma_0} k s(\gamma x_0) (\gamma'(x_0))^{k-1} \gamma''(x_0) \\ &= 1 + \sum_{\gamma \in \Gamma - \Gamma_0} s'(\gamma x_0) (\gamma'(x_0))^k + k \sum_{\gamma \in \Gamma - \Gamma_0} s(\gamma x_0) (\gamma'(x_0))^{k-1} \gamma''(x_0) \end{aligned}$$

so that

$$|g'(x_0) - 1| \leq \sup_{\Delta} |s'(z)| \cdot S\left(\frac{1}{2}\right)^{k-2} + k \sup_{\Delta} |s(z)| \cdot S\left(\frac{1}{2}\right)^{k-3} \cdot C. \quad (3)$$

From (1), (2) and (3), noting that  $\lim_{k \rightarrow \infty} \left(\frac{1}{2}\right)^k = \lim_{k \rightarrow \infty} k \left(\frac{1}{2}\right)^{k-3} = 0$ , we deduce that there exists an integer  $k_1 \geq k_0$  such that for any  $k \geq k_1$  we have

$$|g'(x_0)| \geq \frac{1}{2}, |g(x_0)| \leq \frac{1}{4}, |f'(x_0)| \leq \frac{1}{4}.$$

Since  $|f(x_0)| \geq \frac{1}{2}$  for  $k \geq k_0$ , whenever  $k \geq k_1$  we have

$$|f(x_0)g'(x_0) - g(x_0)f'(x_0)| \geq \frac{1}{2} \cdot \frac{1}{2} - \frac{1}{4} \cdot \frac{1}{4} > 0,$$

so that

$$\left(\frac{g}{f}\right)'(x_0) = \frac{1}{(f(x_0))^2} (f(x_0)g'(x_0) - g(x_0)f'(x_0)) \neq 0,$$

as desired. The proof of the proposition is complete.  $\square$